%!TEX root = forallx.tex
\chapter[Solutions to selected exercises]{Solutions to selected exercises}
\label{app.solutions}

%OL fordítása kezdet

Many of the exercises may be answered correctly in different ways. Where that is the case, the solution here represents one possible correct answer.

Sok feladat megoldását lehet különböző úton/módon megválaszolni. Ahol ez a helyzet, a megoldás csak egy lehetséges helyes választ ad.

\solutionsection{ch.intro}{pr.MartianGiraffes}
\begin{earg}
%\nextSeq %G2, G3, and G4
\item consistent

\item konzisztens
%\noSeq %G1, G3, and G4
\item inconsistent

\item inkonzisztens
%\nextSeq %G1, G2, and G4
\item consistent

\item konzisztens
%\lastSeq %G1, G2, and G3
\item consistent

\item konzisztens
%are consistent.
\end{earg}

\solutionsection{ch.intro}{pr.EnglishCombinations}
%\begin{earg}
%\item A valid argument that has one false premise and one true premise
%possible
\nextSeq
%\item A valid argument that has a false conclusion
%possible
\nextSeq
%\item A valid argument, the conclusion of which is a contradiction
%possible
\nextSeq
%\item An invalid argument, the conclusion of which is a tautology
%not possible
\noSeq
%\item A tautology that is contingent
%not possible
\noSeq
%\item Two logically equivalent sentences, both of which are tautologies
%possible
\nextSeq
%\item Two logically equivalent sentences, one of which is a tautology and one of which is contingent
%not possible
\noSeq
%\item Two logically equivalent sentences that together are an inconsistent set
%possible
\nextSeq
%Consider two contradictions. As a matter of logic, they are both necessarily false. So they have the same truth value: false. This makes them logically equivalent.
%\item A consistent set of sentences that contains a contradiction
%not possible
\noSeq
%\item An inconsistent set of sentences that contains a tautology
%possible
\lastSeq
%\end{earg}
are possible.

lehetségesek.

\solutionsection{ch.SL}{pr.monkeysuits}
\begin{earg}
\item $\enot M$
\item $M \eor \enot M$
\item $G \eor C$
\item $\enot C \eand \enot G$
\item $C \eif (\enot G \eand \enot M)$
\item $M \eor (C \eor G)$
\end{earg}


\solutionsection{ch.SL}{pr.avacareer}
\begin{earg}
\item $E_1 \eand E_2$
\item $F_1 \eif S_1$
\item $F_1 \eor E_1$
\item $E_2 \eand \enot S_2$
\item $\enot E_1 \eand \enot E_2$
\item $E_1 \eand E_2 \eand \enot(S_1 \eor S_2)$
\item $S_2 \eif F_2$
\item $(\enot E_1 \eif \enot E_2) \eand (E_1 \eif E_2)$
\item $S_1 \eiff \enot S_2$
\item $(E_2 \eand F_2) \eif S_2$
\item $\enot(E_2 \eand F_2)$
\item $(F_1 \eand F_2) \eiff (\enot E_1 \eand \enot E_2)$
\end{earg}

\solutionsection{ch.SL}{pr.spies}
\begin{ekey}
\item[A:] Alice is a spy.

\item[A:] Alice egy kém.
\item[B:] Bob is a spy.

\item[B:] Bob egy kém.
\item[C:] The code has been broken.

\item[C:] A kód megsérült.
\item[G:] The German embassy will be in an uproar.

\item[G:] A német nagykövetség felháborodott lesz.
\end{ekey}
\begin{earg}
\item %Alice and Bob are both spies.
$A \eand B$
\item %If either Alice or Bob is a spy, then the code has been broken.
$(A \eor B) \eif C$
\item %If neither Alice nor Bob is a spy, then the code remains unbroken.
$\enot(A \eor B) \eif \enot C$
\item %The German embassy will be in an uproar, unless someone has broken the code.
$G \eor C$
\item %Either the code has been broken or it has not, but the German embassy will be in an uproar regardless.
$(C \eor \enot C) \eand G$
\item %Either Alice or Bob is a spy, but not both.
$(A \eor B) \eand \enot(A \eand B)$
\end{earg}


\solutionsection{ch.SL}{pr.wiffSL}
\begin{earg}
\item %$(A)$
(a) no (b) no

\item %$(A)$
(a) nem (b) nem
\item %$J_{374} \eor \enot J_{374}$
(a) no (b) yes

\item %$J_{374} \eor \enot J_{374}$
(a) nem (b) igen
\item %$\enot \enot \enot \enot F$
(a) yes (b) yes

\item %$\enot \enot \enot \enot F$
(a) igen (b) igen
\item %$\enot \eand S$
(a) no (b) no

\item %$\enot \eand S$
(a) nem (b) nem
\item %$(G \eand \enot G)$
(a) yes (b) yes

\item %$(G \eand \enot G)$
(a) igen (b) igen
\item %$\script{A} \eif \script{A}$
(a) no (b) no

\item %$\script{A} \eif \script{A}$
(a) nem (b) nem
\item %$(A \eif (A \eand \enot F)) \eor (D \eiff E)$
(a) no (b) yes

\item %$(A \eif (A \eand \enot F)) \eor (D \eiff E)$
(a) nem (b) igen
\item %$[(Z \eiff S) \eif W] \eand [J \eor X]$
(a) no (b) yes

\item %$[(Z \eiff S) \eif W] \eand [J \eor X]$
(a) nem (b) igen
\item %$(F \eiff \enot D \eif J) \eor (C \eand D)$
(a) no (b) no

\item %$(F \eiff \enot D \eif J) \eor (C \eand D)$
(a) nem (b) nem
\end{earg}




\solutionsection{ch.TruthTables}{pr.TT.TTorC}
\begin{earg}
\item tautology

\item tautológia
\item contradiction

\item ellentmondás
\item contingent

\item kontingens
\item tautology

\item tautológia
\item tautology

\item tautológia
\item contingent

\item kontingens
\item tautology

\item tautológia
\item contradiction

\item ellentmondás
\item tautology

\item tautológia
\item contradiction

\item ellentmondás
\item tautology

\item tautológia
\item contingent

\item kontingens
\item contradiction

\item ellentmondás
\item contingent

\item kontingens
\item tautology

\item tautológia
\item tautology

\item tautológia
\item contingent

\item kontingens
\item contingent

\item kontingens
\end{earg}

\solutionsection{ch.TruthTables}{pr.TT.equiv}
%\begin{earg}
%\item not equivalent
\noSeq
%\item equivalent
\nextSeq
%\item equivalent
\nextSeq
%\item not equivalent
\noSeq
%\item equivalent
\nextSeq
%\item equivalent
\nextSeq
%\item not equivalent
\noSeq
%\item equivalent
\nextSeq
%\item equivalent
\lastSeq
%\item not equivalent
\noSeq
%\end{earg}
are logically equivalent.

logikailag ekvivalensek.

\solutionsection{ch.TruthTables}{pr.TT.consistent}
%\item $A\eif A$, $\enot A \eif \enot A$, $A\eand A$, $A\eor A$ %consistent
\nextSeq
%\item $A \eand B$, $C\eif \enot B$, $C$ %inconsistent
\noSeq
%\item $A\eor B$, $A\eif C$, $B\eif C$ %consistent
\nextSeq
%\item $A\eif B$, $B\eif C$, $A$, $\enot C$ %inconsistent
\noSeq
%\item $B\eand(C\eor A)$, $A\eif B$, $\enot(B\eor C)$  %inconsistent
\noSeq
%\item $A \eor B$, $B\eor C$, $C\eif \enot A$ %consistent
\nextSeq
%\item $A\eiff(B\eor C)$, $C\eif \enot A$, $A\eif \enot B$ %consistent
\nextSeq
%\item $A$, $B$, $C$, $\enot D$, $\enot E$, $F$ %consistent
\lastSeq
are consistent.

konzisztensek.

\solutionsection{ch.TruthTables}{pr.TT.valid}
%\item $A\eif A$, \therefore\ $A$ %invalid
\noSeq
%\item $A\eor\bigl[A\eif(A\eiff A)\bigr]$, \therefore\ A %invalid
\noSeq
%\item $A\eif(A\eand\enot A)$, \therefore\ $\enot A$ %valid
\nextSeq
%\item $A\eiff\enot(B\eiff A)$, \therefore\ $A$ %invalid
\noSeq
%\item $A\eor(B\eif A)$, \therefore\ $\enot A \eif \enot B$ %valid
\nextSeq
%\item $A\eif B$, $B$, \therefore\ $A$ %invalid
\noSeq
%\item $A\eor B$, $B\eor C$, $\enot A$, \therefore\ $B \eand C$ %invalid
\noSeq
%\item $A\eor B$, $B\eor C$, $\enot B$, \therefore\ $A \eand C$ %valid
\nextSeq
%\item $(B\eand A)\eif C$, $(C\eand A)\eif B$, \therefore\ $(C\eand B)\eif A$ %invalid
\noSeq
%\item $A\eiff B$, $B\eiff C$, \therefore\ $A\eiff C$ %valid
\lastSeq
are valid.

érvényesek.


\solutionsection{ch.TruthTables}{pr.TT.concepts}
\begin{earg}
\item %Suppose that \script{A} and \script{B} are logically equivalent. What can you say about $\script{A}\eiff\script{B}$?
\script{A} and \script{B} have the same truth value on every line of a complete truth table, so $\script{A}\eiff\script{B}$ is true on every line. It is a tautology.

\item %Suppose that \script{A} and \script{B} are logically equivalent. What can you say about $\script{A}\eiff\script{B}$?
\script{A} és \script{B} azonos igazságértékkel rendelkeznek minden sorában a teljes igazságtáblázatban, tehát $\script{A}\eiff\script{B}$ igaz minden sorban. Ez egy tautológia.
\item %Suppose that $(\script{A}\eand\script{B})\eif\script{C}$ is contingent. What can you say about the argument ``\script{A}, \script{B}, \therefore\script{C}''?
The sentence is false on some line of a complete truth table. On that line, \script{A} and \script{B} are true and \script{C} is false. So the argument is invalid.

\item %Suppose that $(\script{A}\eand\script{B})\eif\script{C}$ is contingent. What can you say about the argument ``\script{A}, \script{B}, \therefore\script{C}''?
Az állítás hamis az igazságtáblázat néhány sorában. Ezeken a sorokon, \script{A} és \script{B} igaz és  \script{C} hamis. Tehát az argumentum érvénytelen.
\item %Suppose that $\{\script{A},\script{B}, \script{C}\}$ is inconsistent. What can you say about $(\script{A}\eand\script{B}\eand\script{C})$?
Since there is no line of a complete truth table on which all three sentences are true, the conjunction is false on every line. So it is a contradiction.

\item %Suppose that $\{\script{A},\script{B}, \script{C}\}$ is inconsistent. What can you say about $(\script{A}\eand\script{B}\eand\script{C})$?
Mivel nincs olyan sora a teljes igazságtáblázatnak, melyben mindhárom állítás igaz lenne, a konjukció minden sorban hamis. Tehát ez egy ellentmondás.
\item %Suppose that \script{A} is a contradiction. What can you say about the argument ``\script{A}, \script{B}, \therefore\script{C}''?
Since \script{A} is false on every line of a complete truth table, there is no line on which \script{A} and \script{B} are true and \script{C} is false. So the argument is valid.

\item %Suppose that \script{A} is a contradiction. What can you say about the argument ``\script{A}, \script{B}, \therefore\script{C}''?
Mivel \script{A} hamis a teljes igazságtáblázat minden sorában, nem létezik olyan sor, melyen \script{A} és \script{B} igaz és \script{C} hamis. Tehát az argumentum érvényes.
\item %Suppose that \script{C} is a tautology. What can you say about the argument ``\script{A}, \script{B}, \therefore\script{C}''?
Since \script{C} is true on every line of a complete truth table, there is no line on which \script{A} and \script{B} are true and \script{C} is false. So the argument is valid.

\item %Suppose that \script{C} is a tautology. What can you say about the argument ``\script{A}, \script{B}, \therefore\script{C}''?
Mivel \script{C} igaz a teljes igazságtáblázat minden sorában, nincs olyan sor, melyen \script{A} és \script{B} igaz és \script{C} hamis. Tehát az argumentum érvényes.
\item %Suppose that \script{A} and \script{B} are logically equivalent. What can you say about $(\script{A}\eor\script{B})$?
Not much. $(\script{A}\eor\script{B})$ is a tautology if \script{A} and \script{B} are tautologies; it is a contradiction if they are contradictions; it is contingent if they are contingent.

\item %Suppose that \script{A} and \script{B} are logically equivalent. What can you say about $(\script{A}\eor\script{B})$?
Nem sok. $(\script{A}\eor\script{B})$ egy tautológia, ha \script{A} és \script{B} tautológiák; ellentmondás, ha ellentmondások; kontingens ha kontingensek.
\item %Suppose that \script{A} and \script{B} are \emph{not} logically equivalent. What can you say about $(\script{A}\eor\script{B})$?
\script{A} and \script{B} have different truth values on at least one line of a complete truth table, and $(\script{A}\eor\script{B})$ will be true on that line. On other lines, it might be true or false. So $(\script{A}\eor\script{B})$ is either a tautology or it is contingent; it is \emph{not} a contradiction.

\item %Suppose that \script{A} and \script{B} are \emph{not} logically equivalent. What can you say about $(\script{A}\eor\script{B})$?
\script{A} és \script{B} eltérő igazságértékkel rendelkeznek a teljes igazságtáblázat legalább egy sorában, ezen a soron $(\script{A}\eor\script{B})$ igaz lesz. Más sorokban ez lehet igaz vagy hamis. Tehát $(\script{A}\eor\script{B})$ tautológia vagy kontingens; ez \emph{nem} egy ellentmondás.
\end{earg}

%OL fordítása vége

%LDR fordítása kezdet

\solutionsection{ch.TruthTables}{pr.altConnectives}
\begin{earg}
\item %$A\eor B$
$\enot A \eif B$
\item %$A\eand B$
$\enot(A \eif \enot B)$
\item %$A\eiff B$
$\enot [(A\eif B) \eif \enot(B\eif A)]$
%\item %$A \eand B$
%$\enot(\enot A \eor \enot B)$
%\item %$A \eif B$
%$\enot A \eor B$
%\item %$A \eiff B$
%$\enot(\enot A \eor \enot B) \eor \enot(A \eor B)$
\end{earg}



\solutionsection{ch.QL}{pr.QLalligators}
\begin{earg}
\item %Amos, Bouncer, and Cleo all live at the zoo.
$Za \eand Zb \eand Zc$
\item %Bouncer is a reptile, but not an alligator. 
$Rb \eand \enot Ab$
\item %If Cleo loves Bouncer, then Bouncer is a monkey. 
$Lcb \eif Mb$
\item %If both Bouncer and Cleo are alligators, then Amos loves them both.
$(Ab \eand Ac)\eif(Lab \eand Lac)$
\item %Some reptile lives at the zoo. 
$\exists x(Rx \eand Zx)$
\item %Every alligator is a reptile. 
$\forall x(Ax \eif Rx)$
\item %Any animal that lives at the zoo is either a monkey or an alligator. 
$\forall x\bigl[Zx \eif (Mx \eor Ax)\bigr]$
\item %There are reptiles which are not alligators.
$\exists x(Rx \eand \enot Ax)$
\item %Cleo loves a reptile.
$\exists x(Rx \eand Lcx)$
\item %Bouncer loves all the monkeys that live at the zoo.
$\forall x\bigl[(Mx \eand Zx) \eif Lbx\bigr]$
\item %All the monkeys that Amos loves love him back.
$\forall x\bigl[(Mx \eand Lax) \eif Lxa\bigr]$
\item %If any animal is an reptile, then Amos is.
$\exists x Rx \eif Ra$
\item %If any animal is an alligator, then it is a reptile.
$\forall x(Ax \eif Rx)$
\item %Every monkey that Cleo loves is also loved by Amos.
$\forall x\bigl[(Mx \eand Lcx) \eif Lax\bigr]$
\item %There is a monkey that loves Bouncer, but sadly Bouncer does not reciprocate this love.
$\exists x(Mx \eand Lxb \eand \enot Lbx)$
\end{earg}


\solutionsection{ch.QL}{pr.QLcandies}
\begin{earg}
\item %Boris has never tried any candy.
$\enot\exists x Tx$
\item %Marzipan is always made with sugar.
$\forall x(Mx \eif Sx)$
\item %Some candy is sugar-free.
$\exists x \enot Sx$
\item %The very best candy is chocolate.
$\exists x[Cx \eand \enot\exists y Byx]$
\item %No candy is better than itself.
$\enot \exists x Bxx$
\item %Boris has never tried sugar-free chocolate.
$\enot \exists x(Cx \eand \enot Sx \eand Tx)$
\item %Boris has tried marzipan and chocolate, but never together.
$\exists x(Cx \eand Tx) \eand \exists x(Mx \eand Tx) \eand \enot \exists x(Cx \eand Mx \eand Tx)$
%\item Boris has tried nothing that is better than sugar-free marzipan.
%$\enot\exists x[Bx \eand \exists y(
\item %Any candy with chocolate is better than any candy without it.
$\forall x[Cx \eif \forall y(\enot Cy \eif Bxy)]$
\item %Any candy with chocolate and marzipan is better than any candy without either.
$\forall x\bigl((Cx \eand Mx) \eif \forall y[(\enot Cy \eand \enot My) \eif Bxy]\bigr)$
\end{earg}


\solutionsection{ch.QL}{pr.QLballet}
\begin{earg}
\item %All of Patrick's children are ballet dancers.
$\forall x(Cxp \eif Dx)$
\item %Jane is Patrick's daughter.
$Cjp \eand Fj$
\item %Patrick has a daughter.
$\exists x(Cxp \eand Fx)$
\item %Jane is an only child.
$\enot\exists x Sxj$
\item %All of Patrick's daughters dance ballet.
$\forall x\bigl[(Cxp \eand Fx)\eif Dx\bigr]$
\item %Patrick has no sons.
$\enot\exists x(Cxp \eand Mx)$
\item %Jane is Elmer's niece.
$\exists x(Cjx \eand Sxe \eand Fj)$
\item %Patrick is Elmer's brother.
$Spe \eand Mp$
\item %Patrick's brothers have no children.
$\forall x\bigl[(Sxp \eand Mx) \eif \enot\exists y Cyx\bigr]$
\item %Jane is an aunt.
$\exists x(Sxj \eand \exists y Cyx \eand Fj)$
\item %Everyone who dances in the ballet has a sister who also dances in the ballet.
$\forall x\bigl[Dx \eif \exists y(Sxy \eand Fy \eand Dy)\bigr]$
\item %Every man who dances in the ballet is the child of someone who dances in the ballet.
$\forall x\bigl[(Mx \eand Dx) \eif \exists y(Cxy \eand Dy)\bigr]$
\end{earg}

\solutionsection{ch.QL}{pr.QLcards}
\begin{earg}
\item %All clubs are black cards.
$\forall x(Cx \eif Bx)$
\item %There are no wild cards.
$\enot\exists x Wx$
\item %There are at least two clubs.
$\exists x \exists y(Cx \eand Cy \eand x\neq y)$
\item %There is more than one one-eyed jack.
$\exists x \exists y(Jx \eand Ox \eand Jy \eand Oy \eand x\neq y)$
\item %There are at most two one-eyed jacks.
$\forall x\forall y\forall z\bigl[(Jx \eand Ox \eand Jy \eand Oy \eand Jz \eand Oz)\eif(x=y \eor x=z \eor y=z)\bigr]$
\item %There are two black jacks.
$\exists x\exists y\bigl(Jx \eand Bx \eand Jy \eand By \eand x \neq y\eand \forall z[(Jz \eand Bz) \eif (x=z \eor y=z)]\bigr)$
\item %There are four deuces.
$\exists x_1\exists x_2\exists x_3\exists x_4\bigl[Dx_1 \eand Dx_2 \eand Dx_3 \eand Dx_4 \eand x_1 \neq x_2 \eand x_1 \neq x_3 \eand x_1 \neq x_4 \eand x_2 \neq x_3 \eand x_2 \neq x_4 \eand x_3 \neq x_4  \eand \enot\exists y(Dy \eand y\neq x_1 \eand y\neq x_2 \eand y\neq x_3 \eand y\neq x_4)\bigr]$
\item %The deuce of clubs is a black card.
$\exists x\bigl(Dx \eand Cx \eand \forall y[(Dy\eand Cy) \eif x=y] \eand Bx\bigr)$
\item %One-eyed jacks and the man with the axe are wild.
$\forall x\bigl[(Ox \eand Jx) \eif Wx\bigr] \eand \exists x\bigl[Mx \eand \forall y(My \eif x=y) \eand Wx\bigr]$
\item %If the deuce of clubs is wild, then there is exactly one wild card.
$\exists x\bigl(Dx \eand Cx \eand \forall y[(Dy\eand Cy) \eif x=y] \eand Wx\bigr)\eif \exists x\forall y(Wx \eiff x=y)$
\item %The man with the axe is not a jack.
wide scope: $\enot \exists x\bigl[Mx \eand \forall y(My \eif x=y) \eand Jx\bigr]$\\

tág értelemben: $\enot \exists x\bigl[Mx \eand \forall y(My \eif x=y) \eand Jx\bigr]$\\

narrow scope: $\exists x\bigl[Mx \eand \forall y(My \eif x=y) \eand \enot Jx\bigr]$

szűk értelemben: $\exists x\bigl[Mx \eand \forall y(My \eif x=y) \eand \enot Jx\bigr]$

\item %The deuce of clubs is not the man with the axe.
wide scope: $\enot \exists x\exists z\bigl(Dx \eand Cx \eand Mz \eand \forall y[(Dy\eand Cy) \eif x=y]  \eand \forall y[(My \eif z=y) \eand x=z]\bigr)$\\

tág értelemben: $\enot \exists x\exists z\bigl(Dx \eand Cx \eand Mz \eand \forall y[(Dy\eand Cy) \eif x=y]  \eand \forall y[(My \eif z=y) \eand x=z]\bigr)$\\

narrow scope: $\exists x\exists z\bigl(Dx \eand Cx \eand Mz \eand \forall y[(Dy\eand Cy) \eif x=y]  \eand \forall y[(My \eif z=y) \eand x\neq z]\bigr)$

szűk értelemben: $\exists x\exists z\bigl(Dx \eand Cx \eand Mz \eand \forall y[(Dy\eand Cy) \eif x=y]  \eand \forall y[(My \eif z=y) \eand x\neq z]\bigr)$
\end{earg}





\solutionsection{ch.semantics}{pr.TorF1}
%\item $Bc$
\noSeq
%\item $Ac \eiff \enot Nc$
\nextSeq
%\item $Nc \eif (Ac \eor Bc)$
\nextSeq
%\item $\forall x Ax$
\nextSeq
%\item $\forall x \enot Bx$
\noSeq
%\item $\exists x(Ax \eand Bx)$
\nextSeq
%\item $\exists x(Ax \eif Nx)$
\noSeq
%\item $\forall x(Nx \eor \enot Nx)$
\nextSeq
%\item $\exists x Bx \eif \forall x Ax$
\lastSeq
are true in the model.

igazak a modellben.

\solutionsection{ch.semantics}{pr.TorF2}
\noSeq%\item $\exists x(Rxm \eand Rmx)$
\noSeq%\item $\forall x(Rxm \eor Rmx)$
\noSeq%\item $\forall x(Hx \eiff Wx)$
\nextSeq%\item $\forall x(Rxm \eif Wx)$
\nextSeq%\item $\forall x\bigl[Wx \eif(Hx \eand Wx)\bigr]$
\noSeq%\item $\exists x Rxx$
\lastSeq%\item $\exists x\exists y Rxy$
\noSeq%\item $\forall x \forall y Rxy$
\noSeq%\item $\forall x \forall y (Rxy \eor Ryx)$
\noSeq%\item $\forallx \forall y \forall z\bigl[(Rxy \eand Ryz) \eif Rxz\bigr]$
are true in the model.

igazak a modellben.


\solutionsection{ch.semantics}{pr.InterpretationToModel}
\begin{partialmodel}
UD & \{10,11,12,13\}\\
\extension{O} & \{11,13\}\\
\extension{S} & $\emptyset$\\
\extension{T} & \{10,11,12,13\}\\
\extension{U} & \{13\}\\
\extension{N} & \{\ntuple{11,10},\ntuple{12,11},\ntuple{13,12}\}\\
\end{partialmodel}



\solutionsection{ch.semantics}{pr.Contingent}
\begin{earg}
\item %$Da \eand Db$
	The sentence is true in this model:

	A modellben ez az állítás igaz:

	\begin{partialmodel}
		UD & \{Stan\}\\
		\extension{D} & \{Stan\}\\
		\referent{a} & Stan\\
		\referent{b} & Stan
	\end{partialmodel}

	And it is false in this model:

	És ez hamis a modellben:

	\begin{partialmodel}
		UD & \{Stan\}\\
		\extension{D} & $\emptyset$\\
		\referent{a} & Stan\\
		\referent{b} & Stan
	\end{partialmodel}
\item %$\exists x Txh$

	The sentence is true in this model:

	A modellben ez az állítás igaz:

	\begin{partialmodel}
		UD & \{Stan\}\\
		\extension{T} & \{\ntuple{Stan, Stan}\}\\
		\referent{h} & Stan
	\end{partialmodel}
	And it is false in this model:

	És ez hamis a modellben:
	\begin{partialmodel}
		UD & \{Stan\}\\
		\extension{T} & $\emptyset$\\
		\referent{h} & Stan
	\end{partialmodel}
\item %$Pm \eand \enot\forall x Px$
	The sentence is true in this model:

	A modellben ez az állítás igaz:

	\begin{partialmodel}
		UD & \{Stan, Ollie\}\\
		\extension{P} & \{Stan\}\\
		\referent{m} & Stan
	\end{partialmodel}
	And it is false in this model:

	És ez hamis a modellben:

	\begin{partialmodel}
		UD & \{Stan\}\\
		\extension{P} & $\emptyset$\\
		\referent{m} & Stan
	\end{partialmodel}
\end{earg}



\solutionsection{ch.semantics}{pr.NotEquiv}
There are many possible correct answers. Here are some:

Itt több helyes válasz lehetséges. Itt van néhány közülük:
\begin{earg}
\item %$Ja$, $Ka$
	Making the first sentence true and the second false:

	Így lesz az első mondat igaz, és a második hamis:
	\begin{partialmodel}
		UD & \{alpha\}\\
		\extension{J} & \{alpha\}\\
		\extension{K} & $\emptyset$\\
		\referent{a} & alpha
	\end{partialmodel}
\item %$\exists x Jx$, $Jm$
	Making the first sentence true and the second false:

	Így lesz az első mondat igaz, és a második hamis:
	\begin{partialmodel}
		UD & \{alpha, omega\}\\
		\extension{J} & \{alpha\}\\
		\referent{m} & omega
	\end{partialmodel}
\item %$\forall x Rxx$, $\exists x Rxx$
	Making the first sentence false and the second true:

	Így lesz az első mondat hamis, és a második igaz:
	\begin{partialmodel}
		UD & \{alpha, omega\}\\
		\extension{R} & \{\ntuple{alpha,alpha}\}
	\end{partialmodel}
\item %$\exists x Px \eif Qc$, $\exists x (Px \eif Qc)$
	Making the first sentence false and the second true:

	Így lesz az első mondat hamis, és a második igaz:
	\begin{partialmodel}
		UD & \{alpha, omega\}\\
		\extension{P} & \{alpha\}\\
		\extension{Q} & $\emptyset$\\
		\referent{c} & alpha
	\end{partialmodel}
\item %$\forall x(Px \eif \enot Qx)$, $\exists x(Px \eand \enot Qx)$
	Making the first sentence true and the second false:

	Így lesz az első mondat igaz, és a második hamis:
	\begin{partialmodel}
		UD & \{iota\}\\
		\extension{P} & $\emptyset$\\
		\extension{Q} & $\emptyset$
	\end{partialmodel}
\item %$\exists x(Px \eand Qx)$, $\exists x(Px \eif Qx)$
	Making the first sentence false and the second true:

	Így lesz az első mondat hamis, és a második igaz:
	\begin{partialmodel}
		UD & \{iota\}\\
		\extension{P} & $\emptyset$\\
		\extension{Q} & \{iota\}
	\end{partialmodel}
\item %$\forall x(Px\eif Qx)$, $\forall x(Px \eand Qx)$
	Making the first sentence true and the second false:

	Így lesz az első mondat igaz, és a második hamis:
	\begin{partialmodel}
		UD & \{iota\}\\
		\extension{P} & $\emptyset$\\
		\extension{Q} & \{iota\}
	\end{partialmodel}
\item %$\forall x\exists y Rxy$, $\exists x\forall y Rxy$
	Making the first sentence true and the second false:

	Így lesz az első mondat igaz, és a második hamis:
	\begin{partialmodel}
		UD & \{alpha, omega\}\\
		\extension{R} & \{\ntuple{alpha, omega}, \ntuple{omega, alpha}\}
	\end{partialmodel}
\item %$\forall x\exists y Rxy$, $\forall x\exists y Ryx$
	Making the first sentence false and the second true:

	Így lesz az első mondat hamis, és a második igaz:
	\begin{partialmodel}
		UD & \{alpha, omega\}\\
		\extension{R} & \{\ntuple{alpha, alpha}, \ntuple{alpha, omega}\}
	\end{partialmodel}
\end{earg}

\solutionsection{ch.semantics}{pr.IdentityModels}
\begin{earg}
\item %Show that $\{{\enot}Raa, \forall x (x=a \eor Rxa)\}$ is consistent.
There are many possible answers. Here is one:

Több helyes válasz lehetséges. Az egyik:
\begin{partialmodel}
UD & \{Harry, Sally\}\\
\extension{R} &\{\ntuple{Sally, Harry}\}\\
\referent{a} & Harry
\end{partialmodel}
\item %Show that $\{\forall x\forall y\forall z(x=y \eor y=z \eor x=z), \exists x\exists y\ x\neq y\}$ is consistent.
There are no predicates or constants, so we only need to give a UD.
Any UD with 2 members will do.

Nincsenek predikátumok vagy konstansok, tehát csak egy individuumtartományt kell megadnunk.
Bármelyik két tagú individuumtartomány megteszi.

\item %Show that $\{\forall x\forall y\ x=y, \exists x\ x \neq a\}$ is inconsistent.
We need to show that it is impossible to construct a model in which these are both true. Suppose $\exists x\ x \neq a$ is true in a model. There is something in the universe of discourse that is \emph{not} the referent of $a$. So there are at least two things in the universe of discourse: \referent{a} and this other thing. Call this other thing $\beta$--- we know $a \neq \beta$. But if $a \neq \beta$, then $\forall x\forall y\ x=y$ is false. So the first sentence must be false if the second sentence is true. As such, there is no model in which they are both true. Therefore, they are inconsistent.

Meg kell mutatnunk, hogy nincs olyan modell, amelyikben mindkettő igaz. Tegyük fel, hogy $\exists x\ x \neq a$ igaz a modellben. Van valami az individuumtartományban, ami \emph{nem} az $a$ referense. Tehát van két dolog az individuumtartományban: \referent{a} és ez a másik dolog. Hívjuk ezt a másik dolgot $\beta$-nak. Tudjuk, hogy $a \neq \beta$. De ha $a \neq \beta$, akkor $\forall x\forall y\ x=y$ hamis. Tehát az első mondatnak hamisnak kell lennie, ha ez első igaz. Tehát nincs olyan konzisztens modell, amelyikben mindkettő igaz.

\end{earg}

\solutionsection{ch.semantics}{pr.SemanticsEssay}
\begin{earg}
\stepcounter{eargnum}
\item No, it would not make any difference. The satisfaction of a formula with one or more free variables depends on what the variable assignment does for those variables. Because a sentence has no free variables, however, its satisfaction does not depend on the variable assignment. So a sentence that is satisfied by \emph{some} variable assignment is satisfied by \emph{every} other variable assignment as well.

Nem, ez nem változtatna semmit. A képlet egy vagy több szabad változóval való kielégítése függ attól, hogy mi a változóhozzárendelés azokra a változókra. Mivel, a mondatban nincsenek szabad változók, a kielégítése nem függ a változóhozzárendeléstől. Tehát az az állítás, amit \emph{valamelyik} változóhozzárendelés kielégít, ugyanúgy kielégíti a többi változóhozzárendelés is.
\end{earg}

%LDR fordítása vége

\solutionsection{ch.proofs}{pr.justifySLproof}

\begin{multicols}{2}
\begin{proof}
\hypo{1}{W \eif \enot B}
\hypo{2}{A \eand W}
\hypo{2b}{B \eor (J \eand K)}
\have{3}{W}\ae{2}
\have{4}{\enot B} \ce{1,3}
\have{5}{J \eand K} \oe{2b,4}
\have{6}{K} \ae{5}
\end{proof}

\begin{proof}
\hypo{1}{L \eiff \enot O}
\hypo{2}{L \eor \enot O}
\open
	\hypo{a1}{\enot L}
	\have{a2}{\enot O}\oe{2,a1}
	\have{a3}{L}\be{1,a2}
	\have{a4}{\enot L}\by{R}{a1}
\close
\have{3}{L}\ne{a1-a4}
\end{proof}

\begin{proof}
\hypo{1}{Z \eif (C \eand \enot N)}
\hypo{2}{\enot Z \eif (N \eand \enot C)}
\open
	\hypo{a1}{\enot(N \eor  C)}
	\have{a2}{\enot N \eand \enot C} \by{DeM}{a1}
	\open
		\hypo{b1}{Z} 
		\have{b2}{C \eand \enot N}\ce{1,b1}
		\have{b3}{C}\ae{b2}
		\have{b4}{\enot C}\ae{a2}
	\close
	\have{a3}{\enot Z}\ni{b1-b4}
	\have{a4}{N \eand \enot C}\ce{2,a3}
	\have{a5}{N}\ae{a4}
	\have{a6}{\enot N}\ae{a2}
\close
\have{3}{N \eor C}\ne{a1-a6}
\end{proof}
\end{multicols}

\solutionsection{ch.proofs}{pr.solvedSLproofs}
%Give a proof for each argument in SL.
\begin{earg}
\item%$K\eand L$, \therefore $K\eiff L$
\begin{solutioninlist}
\begin{proof}
	\hypo{a1}{K\eand L} \want{K\eiff L}
	\open
		\hypo{b1}{K} \want{L}
		\have{b2}{L} \ae{a1}
	\close
	\open
		\hypo{c1}{L} \want{K}
		\have{c2}{K} \ae{a1}
	\close
	\have{d1}{K \eiff L} \bi{b1-b2,c1-c2}
\end{proof}
\end{solutioninlist}
\item%$A\eif (B\eif C)$, \therefore $(A\eand B)\eif C$
\begin{solutioninlist}
\begin{proof}
	\hypo{a1}{A\eif (B\eif C)} \want{(A\eand B)\eif C}
	\open
		\hypo{b1}{A\eand B} \want{C}
		\have{b2}{A} \ae{b1}
		\have{b3}{B\eif C} \ce{a1,b2}
		\have{b4}{B} \ae{b1}
		\have{b5}{C} \ce{b3, b4}
	\close
	\have{c}{(A\eand B)\eif C} \ci{b1-b5}
\end{proof}
\end{solutioninlist}
\item%$P \eand (Q\eor R)$, $P\eif \enot R$, \therefore $Q\eor E$
\begin{solutioninlist}
\begin{proof}
	\hypo{a1}{P \eand (Q\eor R)}
	\hypo{a2}{P\eif \enot R} \want{Q\eor E}
	\have{a3}{P} \andE{a1}
	\have{a4}{\enot R} \ifE{a2,a3}
	\have{a5}{Q\eor R} \andE{a1}
	\have{a6}{Q} \orE{a5,a4}
	\have{c}{Q\eor E} \orI{a6}
\end{proof}
\end{solutioninlist}
\item%$(C\eand D)\eor E$, \therefore $E\eor D$
\begin{solutioninlist}
\begin{proof}
	\hypo{a1}{(C\eand D)\eor E} \want{E\eor D}
	\open
		\hypo{b1}{\enot E} \want{D}
		\have{b2}{C\eand D} \oe{a1,b1}
		\have{b3}{D} \ae{b2}
	\close
	\have{c1}{\enot E\eif D} \ci{b1-b3}
	\have{c2}{E\eor D} \by{MC}{c1}
\end{proof}
\end{solutioninlist}
\item%$\enot F\eif G$, $F\eif H$, \therefore $G\eor H$
\begin{solutioninlist}
\begin{proof}
	\hypo{a1}{\enot F\eif G}
	\hypo{a2}{F\eif H} \want{G\eor H}
	\open
		\hypo{b1}{\enot G} \want{H}
		\have{b2}{\enot\enot F} \by{MT}{a1,b1}
		\have{b3}{F} \by{DN}{b2}
		\have{b4}{H} \ce{a2,b3}
	\close
	\have{c1}{\enot G \eif H} \ci{b1-b4}
	\have{c2}{G\eor H} \by{MC}{c1}
\end{proof}
\end{solutioninlist}
\item%$(X\eand Y)\eor(X\eand Z)$, $\enot(X\eand D)$, $D\eor M$ \therefore $M$
\begin{solutioninlist}
\begin{proof}
	\hypo{a1}{(X\eand Y)\eor(X\eand Z)}
	\hypo{a2}{\enot(X\eand D)}
	\hypo{a3}{D\eor M} \want{M}
	\open
		\hypo{b1}{\enot X} \by{for reductio}{}
		\have{b2}{\enot X\eor \enot Y} \oi{b1}
		\have{b3}{\enot (X \eand Y)} \by{DeM}{b2}
		\have{b4}{X\eand Z} \oe{a1,b3}
		\have{b5}{X} \ae{b4}
		\have{b6}{\enot X} \by{R}{b1}
	\close
	\have{c}{X} \ne{b1-b6}
	\open
		\hypo{d1}{\enot M} \by{for reductio}{}
		\have{d2}{D} \oe{a3,d1}
		\have{d3}{X\eand D} \ai{c,d2}
		\have{d4}{\enot(X\eand D)} \by{R}{a2}
	\close
	\have{e}{M} \ne{d1-d4}
\end{proof}
\end{solutioninlist}
\end{earg}


\solutionsection{ch.proofs}{pr.subinstanceQL}
\begin{earg}
\item $Rca$, $Rcb$, $Rcc$, and $Rcd$ are substitution instances of $\forall x Rcx$.
\item Of the expressions listed, only $\forall y Lby$ is a substitution instance of $\exists x\forall y Lxy$.
\end{earg}


\solutionsection{ch.proofs}{pr.justifyQLproof}

\begin{multicols}{2}
%$\{\forall x(\exists y)(Rxy \eor Ryx),\forall x\enot Rmx\}\vdash\exists xRxm$
\begin{proof}
\hypo{p1}{\forall x\exists y(Rxy \eor Ryx)}
\hypo{p2}{\forall x\enot Rmx}
\have{3}{\exists y(Rmy \eor Rym)}\Ae{p1}
	\open
		\hypo{a1}{Rma \eor Ram}
		\have{a2}{\enot Rma}\Ae{p2}
		\have{a3}{Ram}\oe{a1,a2}
		\have{a4}{\exists x Rxm}\Ei{a3}
	\close
\have{n}{\exists x Rxm} \Ee{3,a1-a4}
\end{proof}

%$\{\forall x(\exists yLxy \eif \forall zLzx), Lab\} \vdash \forall xLxx$
\begin{proof}
\hypo{1}{\forall x(\exists yLxy \eif \forall zLzx)}
\hypo{2}{Lab}
\have{3}{\exists y Lay \eif \forall zLza}\Ae{1}
\have{4}{\exists y Lay} \Ei{2}
\have{5}{\forall z Lza} \ce{3,4}
\have{6}{Lca}\Ae{5}
\have{7}{\exists y Lcy \eif \forall zLzc}\Ae{1}
\have{8}{\exists y Lcy}\Ei{6}
\have{9}{\forall z Lzc}\ce{7,8}
\have{10}{Lcc}\Ae{9}
\have{11}{\forall x Lxx}\Ai{10}
\end{proof}

% $\{\forall x(Jx \eif Kx), \exists x\forall y Lxy, \forall x Jx\} \vdash \exists x(Kx \eand Lxx)$
\begin{proof}
\hypo{a}{\forall x(Jx \eif Kx)}
\hypo{b}{\exists x\forall y Lxy}
\hypo{c}{\forall x Jx}
\open
	\hypo{2}{\forall y Lay}
	\have{d}{Ja}\Ae{c}
	\have{e}{Ja \eif Ka}\Ae{a}
	\have{f}{Ka}\ce{e,d}
	\have{3}{Laa}\Ae{2}
	\have{4}{Ka \eand Laa}\ai{f,3}
	\have{5}{\exists x(Kx \eand Lxx)}\Ei{4}
\close
\have{j}{\exists x(Kx \eand Lxx)}\Ee{b,2-5}
\end{proof}


%$\vdash \exists x Mx \eor \forall x\enot Mx$
\begin{proof}
	\open
		\hypo{p1}{\enot (\exists x Mx \eor \forall x\enot Mx)}
		\have{p2}{\enot \exists x Mx \eand \enot \forall x\enot Mx} \by{DeM}{p1}
		\have{p3}{\enot \exists x Mx}\ae{p2}
		\have{p4}{\forall x\enot Mx}\by{QN}{p3}
		\have{p5}{\enot \forall x\enot Mx}\ae{p2}
	\close
\have{n}{\exists x Mx \eor \forall x\enot Mx} \ne{p1-p5}
\end{proof}
\end{multicols}


\solutionsection{ch.proofs}{pr.someQLproofs}

\begin{earg}
\item%$\vdash \forall x Fx \eor \enot \forall x Fx$
\begin{solutioninlist}
\begin{proof}
	\open
		\hypo{p1}{\enot(\forall x Fx \eor \enot\forall x Fx)} \by{for reductio}{}
		\have{s1}{\enot\forall x Fx \eand \enot\enot\forall x Fx} \by{DeM}{p1}
		\have{s2}{\enot \forall x Fx}\ae{s1}
		\have{s3}{\enot\enot\forall x Fx}\ae{s1}
	\close
	\have{c}{\forall x Fx \eor \enot\forall x Fx} \ne{p1-s3}
\end{proof}
\end{solutioninlist}
\item %$\{\forall x(Mx \eiff Nx), Ma\eand\exists x Rxa\}\vdash \exists x Nx$
\begin{solutioninlist}
\begin{proof}
	\hypo{p1}{\forall x(Mx \eiff Nx)}
	\hypo{p2}{Ma \eand \exists x Rxa} \by{want $\exists x Nx$}{}
	\have{a1}{Ma \eiff Na} \Ae{p1}
	\have{a2}{Ma} \ae{p2}
	\have{a3}{Na} \be{a1,a2}
	\have{c}{\exists x Nx} \Ei{a3}
\end{proof}
\end{solutioninlist}
\item %$\{\forall x(\enot Mx \eor Ljx), \forall x(Bx\eif Ljx), \forall x(Mx\eor Bx)\}\vdash \forall xLjx$
\begin{solutioninlist}
\begin{proof}
	\hypo{a1}{\forall x(\enot Mx \eor Ljx)}
	\hypo{a2}{\forall x(Bx \eif Ljx)}
	\hypo{a3}{\forall x(Mx \eor Bx)} \by{want $\forall x Ljx$}{}
	\have{a4}{\enot Ma \eor Lja} \Ae{a1}
	\have{a5}{Ma \eif Lja} \by{MC}{a4}
	\have{a6}{Ba \eif Lja} \Ae{a2}
	\have{a7}{Ma \eor Ba} \Ae{a3}
	\have{a8}{Lja}  \by{DIL}{a7, a5, a6}
	\have{a9}{\forall x Ljx} \Ai{a8}
\end{proof}
\end{solutioninlist}
\item %$\forall x(Cx \eand Dt)\vdash \forall xCx \eand Dt$
\begin{solutioninlist}
\begin{proof}
	\hypo{a1}{\forall x(Cx \eand Dt)} \by{want $\forall x Cx \eand Dt$}{}
	\have{a2}{Ca \eand Dt} \Ae{a1}
	\have{a3}{Ca} \ae{a2}
	\have{a4}{\forall x Cx} \Ai{a3}
	\have{a5}{Dt} \ae{a2}
	\have{a6}{\forall x Cx \eand Dt} \ai{a4, a5}
\end{proof}
\end{solutioninlist}
\item %$\exists x(Cx \eor Dt)\vdash \exists x Cx \eor Dt$
\begin{solutioninlist}
\begin{proof}
	\hypo{a1}{\exists x(Cx \eor Dt)} \by{want $\exists x Cx \eor Dt$}{}
	\open
		\hypo{a2}{Ca \eor Dt} \by{for {$\exists$}E}{}
		\open
			\hypo{a3}{\enot(\exists x Cx \eor Dt)} \by{for reductio}{}
			\have{a4}{\enot\exists x Cx \eand \enot Dt} \by{DeM}{a3}
			\have{a5}{\enot Dt} \ae{a4}
			\have{a6}{Ca} \oe{a2,a5}
			\have{a7}{\exists x Cx} \Ei{a6}
			\have{a8}{\enot\exists x Cx} \ae{a4}
		\close
		\have{a9}{\exists x Cx \eor Dt} \ne{a3-a8}
	\close
	\have{a10}{\exists x Cx \eor Dt} \Ee{a1,a2-a9}
\end{proof}
\end{solutioninlist}
\end{earg}



\solutionsection{ch.proofs}{pr.likes}
Regarding the translation of this argument, see p.~\pageref{likes2}.

\begin{proof}
\hypo{1}{\exists x\forall y[\forall z(Lxz \eif Lyz) \eif Lxy]}
\open
	\hypo{a}{\forall y[\forall z(Laz \eif Lyz) \eif Lay]}
	\have{b}{\forall z(Laz \eif Laz) \eif Laa} \Ae{a}
	\open
		\hypo{c1}{\enot \exists x Lxx} \by{for reductio}{}
		\have{c2}{\forall x\enot Lxx} \by{QN}{c1}
		\have{c3}{\enot Laa} \Ae{c2}
		\have{c4}{\enot \forall z(Laz \eif Laz)} \by{MT}{c2,c3}
		\open
			\hypo{d1}{Lab}
			\have{d2}{Lab} \by{R}{d1}
		\close
		\have{c5}{Lab \eif Lab} \ci{d1--d2}
		\have{c6}{\forall z(Laz \eif Laz)} \Ai{c5}
		\have{cn}{\enot \forall z(Laz \eif Laz)} \by{R}{c4}
	\close
	\have{h}{\exists x Lxx} \ne{c1--cn}
\close
\have{n}{\exists x Lxx} \Ee{1, a--h}
\end{proof}


\solutionsection{ch.proofs}{pr.QLequivornot}
%\item $\forall x Px \eif Qc$, $\forall x (Px \eif Qc)$
\noSeq
%\item $\forall x Px \eand Qc$, $\forall x (Px \eand Qc)$
\nextSeq
%\item $Qc \eor \exists x Qx$, $\exists x (Qc \eor Qx)$
\nextSeq
%\item $\forall x\forall y \forall z Bxyz$, $\forall x Bxxx$
\noSeq
%\item $\forall x\forall y Dxy$, $\forall y\forall x Dxy$
\lastSeq
%\item $\exists x\forall y Dxy$, $\forall y\exists x Dxy$
\noSeq
are logically equivalent.

\solutionsection{ch.proofs}{pr.QLvalidornot}
\noSeq%\item $\forall x\exists y Rxy$, \therefore\ $\exists y\forall x Rxy$
\nextSeq%\item $\exists y\forall x Rxy$, \therefore\ $\forall x\exists y Rxy$
\noSeq%\item $\exists x(Px \eand \enot Qx)$, \therefore\ $\forall x(Px \eif \enot Qx)$
\nextSeq%\item $\forall x(Sx \eif Ta)$, $Sd$, \therefore\ $Ta$
\nextSeq%\item $\forall x(Ax\eif Bx)$, $\forall x(Bx \eif Cx)$, \therefore\ $\forall x(Ax \eif Cx)$
\noSeq%\item $\exists x(Dx \eor Ex)$, $\forall x(Dx \eif Fx)$, \therefore\ $\exists x(Dx \eand Fx)$
\nextSeq%\item $\forall x\forall y(Rxy \eor Ryx)$, \therefore\ $Rjj$
\noSeq%\item $\exists x\exists y(Rxy \eor Ryx)$, \therefore\ $Rjj$
\noSeq%\item $\forall x Px \eif \forall x Qx$, $\exists x \enot Px$, \therefore\ $\exists x \enot Qx$
\lastSeq%\item $\exists x Mx \eif \exists x Nx$, $\enot \exists x Nx$, \therefore\ $\forall x \enot Mx$
are valid. Here are complete answers for some of them:
\begin{earg}
\item %$\forall x\exists y Rxy$, \therefore\ $\exists y\forall x Rxy$
	\begin{solutioninlist}
	\begin{partialmodel}
		UD & \{mocha, freddo\}\\
		\extension{R} & \{\ntuple{mocha, freddo}, \ntuple{freddo, mocha}\}
	\end{partialmodel}
	\end{solutioninlist}
\item %$\exists y\forall x Rxy$, \therefore\ $\forall x\exists y Rxy$
	\begin{solutioninlist}
	\begin{proof}
		\hypo{p}{\exists y\forall x Rxy} \by{want $\forall x\exists y Rxy$}{}
		\open
			\hypo{ass}{\forall x Rxa}
			\have{R}{Rba} \Ae{ass}
			\have{ER}{\exists y Rby} \Ei{R}
			\have{AER}{\forall x \exists y Rxy} \Ai{ER}
		\close
		\have{c}{\forall x\exists y Rxy} \Ee{p, ass-AER}
	\end{proof}
	\end{solutioninlist}
\end{earg}
